Add some basic support for generating schemas for primitive types

jsonstar.fstar.generation.test/SchemaGenerationTests.fs
@@ -1,0 +1,36 @@
+﻿namespace jsonstar.fstar.generation.test
+
+open NUnit.Framework
+open JsonStar_Json
+
+[<TestFixture>]
+type SchemaGenerationTests() = 
+    
+    [<Test>]
+    member this.StringSchema() =
+        let expected_schema_string = """{ "definitions" : {  }, "type" : "string" }"""
+        
+        printfn "%s" SchemaExamples.schema_string
+        Assert.AreEqual(expected_schema_string, SchemaExamples.schema_string)
+
+    [<Test>]
+    member this.IntSchema() =
+        let expected_schema_string = """{ "definitions" : {  }, "type" : "integer" }"""
+        
+        printfn "%s" SchemaExamples.schema_int
+        Assert.AreEqual(expected_schema_string, SchemaExamples.schema_int)
+
+    [<Test>]
+    member this.BoolSchema() =
+        let expected_schema_string = """{ "definitions" : {  }, "type" : "boolean" }"""
+        
+        printfn "%s" SchemaExamples.schema_bool
+        Assert.AreEqual(expected_schema_string, SchemaExamples.schema_bool)
+
+    [<Test>]
+    member this.NatSchema() =
+        let expected_schema_string = """{ "definitions" : {  }, "type" : "integer", "minimum":0 }"""
+          
+        printfn "%s" SchemaExamples.schema_nat
+        Assert.AreEqual(expected_schema_string, SchemaExamples.schema_nat)
+    
