jsonstar.fstar.generation.test/SchemaExamples.fst
@@ -1,0 +1,17 @@
+﻿module SchemaExamples
+
+let schema_string : string = 
+    let s : JsonStar.Schema.schema = (FStar.Tactics.synth_by_tactic (fun () -> JsonStar.Schema.Generation.gen_schema FStar.Tactics.Goal (`string))) in
+    JsonStar.PrettyPrint.stringify (JsonStar.Schema.toJson s)
+
+let schema_int : string = 
+    let s : JsonStar.Schema.schema = (FStar.Tactics.synth_by_tactic (fun () -> JsonStar.Schema.Generation.gen_schema FStar.Tactics.Goal (`int))) in
+    JsonStar.PrettyPrint.stringify (JsonStar.Schema.toJson s)
+
+let schema_bool : string = 
+    let s : JsonStar.Schema.schema = (FStar.Tactics.synth_by_tactic (fun () -> JsonStar.Schema.Generation.gen_schema FStar.Tactics.Goal (`bool))) in
+    JsonStar.PrettyPrint.stringify (JsonStar.Schema.toJson s)
+
+let schema_nat : string = 
+    let s : JsonStar.Schema.schema = (FStar.Tactics.synth_by_tactic (fun () -> JsonStar.Schema.Generation.gen_schema FStar.Tactics.Goal (`nat))) in
+    JsonStar.PrettyPrint.stringify (JsonStar.Schema.toJson s)
