jsonstar/JsonStar.Schema.Generation.Api.fst
@@ -3,3 +3,5 @@ module JsonStar.Schema.Generation.Api
 open JsonStar.Schema
 
 let string_s : schema = FStar.Tactics.synth_by_tactic (fun () -> JsonStar.Schema.Generation.gen_schema FStar.Tactics.Goal (`string))
+
+let nat_s : schema = FStar.Tactics.synth_by_tactic (fun () -> JsonStar.Schema.Generation.gen_schema FStar.Tactics.Goal (`nat))
