jsonstar/JsonStar.Schema.Generation.Attributes.fst
@@ -1,0 +1,2 @@
+module JsonStar.Schema.Generation.Attributes
+
