jsonstar/JsonStar.Schema.Generation.Helpers.fst
@@ -1,0 +1,26 @@
+module JsonStar.Schema.Generation.Helpers
+
+module T = FStar.Tactics
+module L = FStar.List.Tot
+
+let tfail (#a: Type) (s:string) : T.Tac a =
+    T.debug ("Tactic failure: " ^ s);
+    T.fail s
+
+let rec app_head_rev_tail (t: T.term) : T.Tac (T.term * list T.argv) =
+    let ins = T.inspect t in
+    if T.Tv_App? ins
+    then 
+        let (T.Tv_App u v) = ins in
+        let (x, l) = app_head_rev_tail u in
+        (x, v :: l)
+    else (t, [])
+
+// Tactic that extracts a term and potentially it's arguments if it's a function application
+let app_head_tail (t : T.term) : T.Tac (T.term * list T.argv) =
+    let (x,l) = app_head_rev_tail t in
+    (x, L.rev l)
+
+let drop_synonym (e : T.env) (t : T.term) : T.Tac (T.term) =
+    // delta normalization unfolds names
+    T.norm_term_env e [delta] t
