jsonstar/JsonStar.Schema.Generation.Primitive.fst
@@ -1,0 +1,31 @@
+module JsonStar.Schema.Generation.Primitive
+
+module T = FStar.Tactics
+module L = FStar.List.Tot
+
+//module Helpers = JsonStar.Schema.Generation.Helpers
+
+open JsonStar.Schema
+
+let primitives = [ "Prims.string"; "Prims.int"; "Prims.bool" ]
+let isPrimitive (tv : T.term_view) : Tot bool =
+    match tv with
+    | T.Tv_FVar fv -> L.mem (T.fv_to_string fv) primitives
+    | _          -> false
+
+let mkPrimitiveSchema (s : schema_type) : Tot schema = 
+    {
+        _id = None;
+        _schema = None;
+        _type = s;
+        description = None;
+        title = None;
+        _default = None;
+        definitions = [];
+    }
+
+let toSchema (t : T.term) : T.Tac (option schema) =
+    if T.term_eq t (`string) then Some (mkPrimitiveSchema (String (mkempty_string_options ())))
+    else if T.term_eq t (`int) then Some (mkPrimitiveSchema Integer)
+    else if T.term_eq t (`bool) then Some (mkPrimitiveSchema Boolean)
+    else None
