jsonstar/JsonStar.Schema.Generation.Refinement.fst
@@ -1,0 +1,43 @@
+module JsonStar.Schema.Generation.Refinement
+
+module T = FStar.Tactics
+module L = FStar.List.Tot
+
+open JsonStar.Schema
+
+// Refinement recognizer
+let isRefinement (tv : T.term_view) : Tot bool = 
+    match tv with
+    | T.Tv_Refine _ _ -> true
+    | _           -> false
+
+// Split refinement over "and"
+
+// Some common refinements recognizers? Like >=, >, <, <=?
+// TODO: I think we have two kinds of refinements:
+//       1. Defined as a bool predicate
+//       2. Defined as a "Type" predicate
+//       We should recognize and unpack both. At that point we should split by "and" and look for known pieces of
+//       code. 
+
+type refinement = 
+    | Minimum : v:int -> refinement
+    | Maximum : v:int -> refinement
+
+// nat
+//Tv_Refine 
+//  (
+//    (i:Prims.int), 
+//    Tv_App 
+//      (
+//        Tv_App 
+//          (
+//            Tv_App 
+//              (
+//                Tv_FVar Prims.eq2, 
+//                Tv_FVar Prims.bool
+//              ), 
+//                Tv_App (Tv_App (Tv_FVar Prims.op_GreaterThanOrEqual, Tv_Var (i:Prims.int)), C_Int 0)
+//          ), C_True
+//      )
+//  )
