jsonstar/JsonStar.Schema.Generation.fst
@@ -10,14 +10,12 @@ let s : schema = T.synth_by_tactic (fun () -> gen_schema T.Goal (`string))
 *)
 module JsonStar.Schema.Generation
 
-// TODO: Fix F# compilation (requires FStar.Tactics in ulib?)
 // TODO: Create a DSL for describing supported refinements? 
 //       Or maybe it would be better to parameterize gen_schema with a list of 
 //       "converters" for handling refinements in types? 
 //       I don't think we can handle arbitrary refinements for schema generation.
 
 open FStar.String
-open FStar.Tactics
 
 module T = FStar.Tactics
 module L = FStar.List.Tot
@@ -26,41 +24,29 @@ open JsonStar.Schema
 open JsonStar.Json
 open JsonStar.PrettyPrint
 
-let tfail (#a: Type) (s:string) : T.Tac a =
-    T.debug ("Tactic failure: " ^ s);
-    T.fail s
+module Helpers = JsonStar.Schema.Generation.Helpers
+module Primitive = JsonStar.Schema.Generation.Primitive
+module Refinement = JsonStar.Schema.Generation.Refinement
 
-let rec app_head_rev_tail (t: T.term) : T.Tac (T.term * list T.argv) =
-    let ins = T.inspect t in
-    if T.Tv_App? ins
-    then 
-        let (T.Tv_App u v) = ins in
-        let (x, l) = app_head_rev_tail u in
-        (x, v :: l)
-    else (t, [])
+open FStar.Reflection.Data
 
-// Tactic that extracts a term and potentially it's arguments if it's a function application
-let app_head_tail (t : T.term) : T.Tac (T.term * list T.argv) =
-    let (x,l) = app_head_rev_tail t in
-    (x, L.rev l)
+let refinementToSchema (t : T.term) : T.Tac (option schema) = 
+    match T.inspect t with
+    | T.Tv_Refine b phi ->
+        let b = T.inspect_bv b in
+        let baseTerm : T.term = b.bv_sort in
+        // TODO: Handle refinements
+        Primitive.toSchema baseTerm
+    | _ -> Helpers.tfail ("Expected " ^ (T.term_to_string t) ^ " to be refinement")
 
-let drop_synonym (e : env) (t : T.term) : T.Tac (T.term) =
-    // delta normalization unfolds names
-    norm_term_env e [delta] t
-
-// TODO: Not implemented yet
 let tryGenSchema (t : T.term) : T.Tac (option schema) = 
-    //None
-    Some 
-        ({
-            _id = None;
-            _schema = None;
-            _type = String (mkempty_string_options ());
-            description = None;
-            title = None;
-            _default = None;
-            definitions = [];
-        })
+    let ast = FStar.Tactics.Print.term_to_ast_string t in
+    T.print ast;
+    
+    let tv : T.term_view = T.inspect t in
+    if Primitive.isPrimitive tv then Primitive.toSchema t
+    else if Refinement.isRefinement tv then refinementToSchema tv
+    else None
 
 /// Schema generation tactic
 /// @ignore_synonyms - replace type abbreviations with its definition
@@ -68,23 +54,23 @@ let tryGenSchema (t : T.term) : T.Tac (option schema) =
 let gen_schema' (ignore_synonyms : bool) (typ: T.term) : T.Tac (T.term) =
     let t = 
         if ignore_synonyms
-            then drop_synonym (top_env()) typ
-            else fst (app_head_tail typ)
+            then Helpers.drop_synonym (T.top_env()) typ
+            else fst (Helpers.app_head_tail typ)
     in
     let s : option schema = tryGenSchema t in
 
     match s with
     | Some s' -> quote s'
-    | None -> tfail ("Unsupported type while generating schema:\n" ^ (term_to_string typ) ^ "\n")
+    | None -> Helpers.tfail ("Unsupported type while generating schema:\n" ^ (T.term_to_string typ) ^ "\n")
 
 let gen_schema (pol: T.guard_policy) (t:T.term) : T.Tac unit =
     let s = gen_schema' true t in
     // Somehow, this line causes the tactic to get stuck when actually trying to print it.
     // Either with T.print, or T.debug with debug flag is enabled. 
-    let s_string : string = JsonStar.PrettyPrint.stringify (toJson (unquote s)) in
+    let s_string : string = JsonStar.PrettyPrint.stringify (toJson (T.unquote s)) in
     // F* prints the stringified result when run with 
     // [--debug JsonStar.Schema.Generation --debug_level Tac] flags. 
     // It's rather verbose. For now we just use print.
     //T.print s_string;
-    T.debug ("Schema produced for (" ^ (term_to_string t) ^ "):\n" ^ s_string ^ "\n");
-    exact_guard s
+    T.debug ("Schema produced for (" ^ (T.term_to_string t) ^ "):\n" ^ s_string ^ "\n");
+    T.exact_guard s
